rocq/BST.v
@@ -164,7 +164,7 @@ Print Assumptions G0_ok.
     stated over, and the next rule cannot start. *)
 
 Section bst.
-  Context `{!rcuG Σ, !physG Σ, !heapG Σ, !lockG Σ, !stackG Σ, !freshG Σ,
+  Context `{!rcuG Σ, !physG Σ, !readerG Σ, !heapG Σ, !lockG Σ, !stackG Σ, !freshG Σ,
             !invGS_gen hlc Σ}.
   Context (FType : FName -> FieldKind).
   Hypothesis HFs : forall g, FType g = RCUField -> In g Fs.
@@ -177,9 +177,9 @@ Section bst.
   Definition U1 : Var -> TID -> Prop :=
     fun y t => U0 y t /\ (y, t) <> (vCurrentF, W).
 
-  Lemma bst_alloc N γm γh γl γs γo γf γr E :
+  Lemma bst_alloc N γm γh γl γs γd γo γf γr E :
     ↑N ⊆ E ->
-    rcu_invT FType (phys γm γh γl γs Rt Fs) N γo γf γr -∗
+    rcu_invT FType (phys γm γh γl γs γd Rt Fs) N γo γf γr -∗
     writer γo γs γh γl γf W Sm0 Ob0 C0 ∅ -∗
     fr_frag γr ∅
     ={E}=∗ ∃ n,
@@ -197,7 +197,7 @@ Section bst.
            ((vCurrentF, TFresh (fun _ => None)) :: G0)⌝.
   Proof.
     iIntros (HN) "#Hinv Hw Hfr".
-    iMod (alloc_typed FType Rt Fs N γm γh γl γs γo γf γr E W vCurrentF Rt
+    iMod (alloc_typed FType Rt Fs N γm γh γl γs γd γo γf γr E W vCurrentF Rt
             U0 Sm0 Ob0 C0 ∅ ∅ (fun _ _ => VNull) G0 HN
             with "Hinv Hw Hfr")
       as (n) "(Hw & Hfr & %Hnr & %Hcn & %Hon & %Hsn & %HFrC & %Hok)".
@@ -249,12 +249,12 @@ Section bst.
     destruct Hc as [Hc | Hc]; [discriminate | by apply not_elem_of_nil in Hc].
   Qed.
 
-  Lemma bst_write_right N γm γh γl γs γo γf γr E n :
+  Lemma bst_write_right N γm γh γl γs γd γo γf γr E n :
     ↑N ⊆ E ->
     n <> Rt ->
     (forall k v, C0 !! k = Some v -> k.1 <> n) ->
     (forall o sg, Ob0 !! o = Some sg -> o <> n) ->
-    rcu_invT FType (phys γm γh γl γs Rt Fs) N γo γf γr -∗
+    rcu_invT FType (phys γm γh γl γs γd Rt Fs) N γo γf γr -∗
     writer γo γs γh γl γf W
       (<[(vCurrentF, W) := n]> Sm0) (<[n := {[Ofresh W]}]> Ob0)
       (newcells Fs n ∪ C0) ∅ -∗
@@ -275,7 +275,7 @@ Section bst.
     iIntros (HN Hnr Hcn Hon) "#Hinv Hw %Hok".
     assert (HnL : n <> LmP)
       by (intros ->; by apply (Hon LmP {[Oiter W]} eq_refl)).
-    iMod (write_fresh_typed FType Rt Fs N γm γh γl γs γo γf γr E W
+    iMod (write_fresh_typed FType Rt Fs N γm γh γl γs γd γo γf γr E W
             vCurrentF vLmParent n Rgt LmP Lft U1
             (<[(vCurrentF, W) := n]> Sm0) (<[n := {[Ofresh W]}]> Ob0)
             (newcells Fs n ∪ C0) ∅ {[Ofresh W]} {[Oiter W]} VNull VNull
@@ -339,12 +339,12 @@ Section bst.
       [currentF.Left = currentL].  The same rule again, and this time its field
       map is not empty -- the entry written in step two has to be carried
       across, which is what the field-map condition is for. *)
-  Lemma bst_write_left N γm γh γl γs γo γf γr E n :
+  Lemma bst_write_left N γm γh γl γs γd γo γf γr E n :
     ↑N ⊆ E ->
     n <> Rt ->
     (forall k v, C0 !! k = Some v -> k.1 <> n) ->
     (forall o sg, Ob0 !! o = Some sg -> o <> n) ->
-    rcu_invT FType (phys γm γh γl γs Rt Fs) N γo γf γr -∗
+    rcu_invT FType (phys γm γh γl γs γd Rt Fs) N γo γf γr -∗
     writer γo γs γh γl γf W
       (<[(vCurrentF, W) := n]> Sm0) (<[n := {[Ofresh W]}]> Ob0)
       (<[(n, Rgt) := VLoc LmP]> (newcells Fs n ∪ C0)) ∅ -∗
@@ -374,7 +374,7 @@ Section bst.
     assert (HnL : n <> LmP) by (intros ->; by apply (Hon LmP {[Oiter W]} eq_refl)).
     assert (HnCL : n <> CurL)
       by (intros ->; by apply (Hon CurL {[Oiter W]} eq_refl)).
-    iMod (write_fresh_typed FType Rt Fs N γm γh γl γs γo γf γr E W
+    iMod (write_fresh_typed FType Rt Fs N γm γh γl γs γd γo γf γr E W
             vCurrentF vCurrentL n Lft CurL Lft U1
             (<[(vCurrentF, W) := n]> Sm0) (<[n := {[Ofresh W]}]> Ob0)
             (<[(n, Rgt) := VLoc LmP]> (newcells Fs n ∪ C0)) ∅
@@ -459,9 +459,9 @@ Section bst.
 
       This is what the exercise was for: one rule's postcondition handed
       directly to the next. *)
-  Lemma bst_build_replacement N γm γh γl γs γo γf γr E :
+  Lemma bst_build_replacement N γm γh γl γs γd γo γf γr E :
     ↑N ⊆ E ->
-    rcu_invT FType (phys γm γh γl γs Rt Fs) N γo γf γr -∗
+    rcu_invT FType (phys γm γh γl γs γd Rt Fs) N γo γf γr -∗
     writer γo γs γh γl γf W Sm0 Ob0 C0 ∅ -∗
     fr_frag γr ∅
     ={E}=∗ ∃ n,
@@ -484,13 +484,13 @@ Section bst.
                                     else None))] ++ G0)⌝.
   Proof.
     iIntros (HN) "#Hinv Hw Hfr".
-    iMod (bst_alloc N γm γh γl γs γo γf γr E HN with "Hinv Hw Hfr")
+    iMod (bst_alloc N γm γh γl γs γd γo γf γr E HN with "Hinv Hw Hfr")
       as (n) "(%Hnr & %Hcn & %Hon & %Hsn & Hw & Hfr & %Hok)".
-    iMod (bst_write_right N γm γh γl γs γo γf γr E n HN Hnr Hcn Hon
+    iMod (bst_write_right N γm γh γl γs γd γo γf γr E n HN Hnr Hcn Hon
             with "Hinv Hw []") as "(Hw & %Hok2)".
     { iPureIntro. intros y ty Hin. apply Hok.
       destruct Hin as [Heq | Hin]; [by left | by right]. }
-    iMod (bst_write_left N γm γh γl γs γo γf γr E n HN Hnr Hcn Hon
+    iMod (bst_write_left N γm γh γl γs γd γo γf γr E n HN Hnr Hcn Hon
             with "Hinv Hw []") as "(Hw & %Hok3)".
     { by iPureIntro. }
     iModIntro. iExists n. iFrame. by iPureIntro.
@@ -570,7 +570,7 @@ Print Assumptions bst_build_replacement.
     here. *)
 
 Section bst4.
-  Context `{!rcuG Σ, !physG Σ, !heapG Σ, !lockG Σ, !stackG Σ, !freshG Σ,
+  Context `{!rcuG Σ, !physG Σ, !readerG Σ, !heapG Σ, !lockG Σ, !stackG Σ, !freshG Σ,
             !invGS_gen hlc Σ}.
   Context (FType : FName -> FieldKind).
 
@@ -781,12 +781,12 @@ Section bst4.
 
       [parent.Left = currentF].  Every side condition is a lookup in a concrete
       map or one of the three distinctness facts above. *)
-  Lemma bst_replace N γm γh γl γs γo γf γr E n :
+  Lemma bst_replace N γm γh γl γs γd γo γf γr E n :
     ↑N ⊆ E ->
     n <> Rt ->
     (forall k v, C0 !! k = Some v -> k.1 <> n) ->
     EnvOK Rt W U1 FType Fs (Sm1 n) (Ob1 n) (C3 n) ∅ Grest ->
-    rcu_invT FType (phys γm γh γl γs Rt Fs) N γo γf γr -∗
+    rcu_invT FType (phys γm γh γl γs γd Rt Fs) N γo γf γr -∗
     writer γo γs γh γl γf W (Sm1 n) (Ob1 n) (C3 n) ∅ -∗
     fr_frag γr ({[n]} : gset Loc)
     ={E}=∗ writer γo γs γh γl γf W (Sm1 n)
@@ -804,7 +804,7 @@ Section bst4.
   Proof.
     iIntros (HN Hr Hcn Hrest) "#Hinv Hw Hfr".
     destruct (n_fresh n Hcn) as (Hc & Hcl & Hlm).
-    iApply (replace_typed FType Rt Fs N γm γh γl γs γo γf γr E W
+    iApply (replace_typed FType Rt Fs N γm γh γl γs γd γo γf γr E W
               vParent vCurrentF vCurrent Rt Lft Cur n [] Lft
               U1 (Sm1 n) (Ob1 n) (C3 n) ∅ {[n]} (Val3 n) Valo
               {[Oiter W]} Grest
@@ -861,11 +861,11 @@ Section bst4.
       triples could not be read off from -- each step's output is the next
       step's input, including the freshness facts the allocation has to export
       and the mirror condition the splice has to be handed. *)
-  Lemma bst_delete_two_child N γm γh γl γs γo γf γr E :
+  Lemma bst_delete_two_child N γm γh γl γs γd γo γf γr E :
     (forall g, FType g = RCUField -> In g Fs) ->
     (forall g, In g Fs -> FType g = RCUField) ->
     ↑N ⊆ E ->
-    rcu_invT FType (phys γm γh γl γs Rt Fs) N γo γf γr -∗
+    rcu_invT FType (phys γm γh γl γs γd Rt Fs) N γo γf γr -∗
     writer γo γs γh γl γf W Sm0 Ob0 C0 ∅ -∗
     fr_frag γr ∅
     ={E}=∗ ∃ n,
@@ -883,14 +883,14 @@ Section bst4.
              (vCurrent, TUnlinked)] ++ Grest)⌝.
   Proof.
     iIntros (HFs HFrcu HN) "#Hinv Hw Hfr".
-    iMod (bst_build_replacement FType HFs HFrcu N γm γh γl γs γo γf γr E HN
+    iMod (bst_build_replacement FType HFs HFrcu N γm γh γl γs γd γo γf γr E HN
             with "Hinv Hw Hfr") as (n) "(%Hr & %Hcn & Hw & Hfr & %Hok)".
     assert (Hrest : EnvOK Rt W U1 FType Fs (Sm1 n) (Ob1 n) (C3 n) ∅ Grest).
     { intros x ty Hin. apply Hok.
       destruct Hin as [Heq | [Heq | []]]; rewrite -Heq;
         [ by right; right; right; left
         | by right; right; right; right; left ]. }
-    iMod (bst_replace N γm γh γl γs γo γf γr E n HN Hr Hcn Hrest
+    iMod (bst_replace N γm γh γl γs γd γo γf γr E n HN Hr Hcn Hrest
             with "Hinv Hw Hfr") as "Hres".
     iModIntro. by iExists n.
   Qed.
